Unifing files in one

src/PriorityQueue.v
@@ -1,31 +1,71 @@
 Module Type PRIQUEUE.
   Definition key := nat.
-  Parameter perm: list key -> list key -> Prop.
   Parameter priqueue: Type.
   Parameter permutation: list key  -> list key  -> Prop.
-
   Parameter empty : priqueue.
   Parameter insert: key -> priqueue -> priqueue.
   Parameter delete_min: priqueue -> option (key * priqueue).
-  Parameter merge: priqueue -> priqueue -> priqueue. 
-  
-  Parameter exist: priqueue -> Prop.
-  Parameter len: priqueue -> list key -> Prop.
-  Axiom can_relate: forall p, exist p -> exists al, len p al.
+  Parameter merge: priqueue -> priqueue -> priqueue.
+  Parameter priq: priqueue -> Prop.
+  Parameter Abs: priqueue -> list key -> Prop.
+
+  Axiom can_relate: forall p, priq p -> exists al, Abs p al.
   Axiom abs_perm: forall p al bl,
-   exist p -> len p al -> len p bl -> permutation al bl.
-  Axiom empty_priq: exist empty.
-  Axiom empty_relate: len empty nil.
-  Axiom insert_priq: forall k p, exist p -> exist (insert k p).
+   priq p -> Abs p al -> Abs p bl -> permutation al bl.
+  Axiom empty_priq: priq empty.
+  Axiom empty_relate: Abs empty nil.
+  Axiom insert_priq: forall k p, priq p -> priq (insert k p).
   Axiom insert_relate:
-        forall p al k, exist p -> len p al -> len (insert k p) (k::al).
+        forall p al k, priq p -> Abs p al -> Abs (insert k p) (k::al).
   Axiom delete_min_None_relate:
-        forall p, exist p -> (len p nil <-> delete_min p = None).
-  Axiom merge_priq: forall p q, exist p -> exist q -> exist (merge p q).
+        forall p, priq p -> (Abs p nil <-> delete_min p = None).
+  Axiom merge_priq: forall p q, priq p -> priq q -> priq (merge p q).
   Axiom merge_relate:
     forall p q pl ql al,
-       exist p -> exist q ->
-       len p pl -> len q ql -> len (merge p q) al ->
+       priq p -> priq q ->
+       Abs p pl -> Abs q ql -> Abs (merge p q) al ->
        permutation al (pl++ql).
 
 End PRIQUEUE.
+
+Require Import List.
+
+Module CartesianTree <: PRIQUEUE.
+  
+  Definition key := nat.
+  Definition insert:= ct_insert.
+  Definition priqueue: .
+  Definition permutation: .
+  Definition empty : .
+
+  Definition delete_min: .
+  Definition merge: .
+  Definition priq: .
+  Definition Abs: .
+
+  Inductive tree : Type :=
+  | leaf : tree
+  | node : nat -> tree -> tree -> tree.
+
+  Definition create_cartesian_tree : list nat -> tree.
+  Admitted.
+
+  Definition ct_insert : nat -> tree -> tree.
+  Admitted.
+
+  Definition delete_min : tree -> tree.
+  Admitted.
+
+  Definition merge : tree -> tree -> tree.
+  Admitted.
+
+  Definition empty : tree := leaf.
+  Admitted.
+
+  Definition flatten : tree -> list nat.
+  Admitted.
+
+  Theorem in_order_traversal : forall (l : list nat), (l = (flatten (create_cartesian_tree l))).
+  Proof. Admitted.
+
+End CartesianTree.
